veric/binop_lemmas4.v
@@ -69,7 +69,7 @@ Proof.
   unfold denote_tc_test_eq in H; simpl in H.
   destruct v; try solve [inv H]; destruct Archi.ptr64; try solve [inv H];
    simpl in H; destruct H; subst;
-   apply Int.eq_true.
+   try apply Int.eq_true; apply Int64.eq_true.
 Qed.
 
 Lemma denote_tc_test_eq_Vlong_r': forall m i v,
@@ -80,9 +80,8 @@ Proof.
   unfold denote_tc_test_eq in H; simpl in H.
   destruct v; try solve [inv H];  destruct Archi.ptr64; try solve [inv H];
   simpl in H; destruct H; subst;
-   apply Int.eq_true.
+   try apply Int.eq_true; apply Int64.eq_true.
 Qed.
-
 
 Lemma denote_tc_test_order_eqblock:
   forall phi b0 i0 b i,
@@ -169,14 +168,14 @@ unfold denote_tc_test_eq in H.
 *
  simpl.
  destruct Archi.ptr64; try contradiction.
- destruct H.  hnf in H. subst i; rewrite Int.eq_true. simpl.
+ destruct H.  hnf in H. subst i; rewrite ?Int.eq_true, ?Int64.eq_true. simpl.
  apply weak_valid_pointer_dry in H0.
  rewrite H0.
  destruct OP; subst; simpl; auto.
 *
  simpl.
  destruct Archi.ptr64; try contradiction.
- destruct H.  hnf in H. subst; rewrite Int.eq_true. simpl.
+ destruct H.  hnf in H. subst; rewrite ?Int.eq_true, ?Int64.eq_true. simpl.
  apply weak_valid_pointer_dry in H0.
  rewrite H0.
  destruct OP; subst; simpl; auto.
@@ -360,27 +359,43 @@ unfold denote_tc_test_eq in *.
 unfold Vptrofs, ptrofs_of_int in *.
 destruct v; try contradiction;
 destruct Archi.ptr64 eqn:Hp; try contradiction; subst.
+-
 destruct H; split; auto.
 clear H.
 hnf in H0|-*.
 destruct si; auto.
+*
 unfold Ptrofs.of_ints in *.
-unfold Ptrofs.to_int in *.
-rewrite (Ptrofs.agree32_repr Hp), Int.repr_unsigned  in H0.
-assert (i = Int.zero) by (rewrite <- (Int.repr_signed i); auto).
+unfold Ptrofs.to_int, Ptrofs.to_int64 in *.
+rewrite ?Ptrofs.agree32_repr, ?Ptrofs.agree64_repr,
+             ?Int.repr_unsigned, ?Int64.repr_unsigned in H0 by auto.
+assert (i=Int.zero)
+  by first [apply Int64repr_Intsigned_zero; solve [auto]
+              | rewrite <- (Int.repr_signed i); auto].
 subst i.
 destruct si'; auto.
+*
 destruct si'; auto.
 unfold Ptrofs.of_intu in H0.
-rewrite Ptrofs.to_int_of_int in H0 by auto.
-subst.
-unfold Ptrofs.of_ints.
-rewrite Int.signed_zero.
-unfold Ptrofs.to_int.
-rewrite Ptrofs.unsigned_repr.
-reflexivity.
-unfold Ptrofs.max_unsigned. rewrite (Ptrofs.modulus_eq32 Hp).
-compute; split; congruence.
+try ( (* Archi.ptr64=false case *)
+ rewrite Ptrofs.to_int_of_int in H0 by auto;
+ subst;
+ unfold Ptrofs.of_ints;
+ rewrite Int.signed_zero;
+ unfold Ptrofs.to_int;
+ rewrite Ptrofs.unsigned_repr; [reflexivity |];
+ unfold Ptrofs.max_unsigned; rewrite (Ptrofs.modulus_eq32 Hp);
+ compute; split; congruence).
+(* Archi.ptr64=true case *)
+unfold Ptrofs.of_int, Ptrofs.to_int64 in H0;
+rewrite Ptrofs.unsigned_repr in H0;
+ [apply Int64repr_Intunsigned_zero in H0; subst; reflexivity
+ | pose proof (Int.unsigned_range i);
+   destruct H; split; auto;
+   assert (Int.modulus < Ptrofs.max_unsigned)
+     by (unfold Ptrofs.max_unsigned, Ptrofs.modulus, Ptrofs.wordsize, Wordsize_Ptrofs.wordsize; rewrite Hp; compute; auto);
+    omega].
+-
 destruct H.
 split; auto.
 hnf in H|-*. clear H0.
@@ -399,7 +414,7 @@ rewrite (Ptrofs.agree64_repr Hp) in H.
 rewrite Int64.repr_unsigned in H.
 apply Int64repr_Intunsigned_zero in H. subst.
 reflexivity.
-*
+-
 destruct H.
 split; auto.
 hnf in H|-*. clear H0.
@@ -421,27 +436,43 @@ unfold denote_tc_test_eq in *.
 unfold Vptrofs, ptrofs_of_int in *.
 destruct v; try contradiction;
 destruct Archi.ptr64 eqn:Hp; try contradiction; subst.
+-
 destruct H; split; auto.
 clear H0.
 hnf in H|-*.
 destruct si; auto.
+*
 unfold Ptrofs.of_ints in *.
-unfold Ptrofs.to_int in *.
-rewrite (Ptrofs.agree32_repr Hp), Int.repr_unsigned  in H.
-assert (i = Int.zero) by (rewrite <- (Int.repr_signed i); auto).
+unfold Ptrofs.to_int, Ptrofs.to_int64 in *.
+rewrite ?Ptrofs.agree32_repr, ?Ptrofs.agree64_repr,
+             ?Int.repr_unsigned, ?Int64.repr_unsigned in H by auto.
+assert (i=Int.zero)
+  by first [apply Int64repr_Intsigned_zero; solve [auto]
+              | rewrite <- (Int.repr_signed i); auto].
 subst i.
 destruct si'; auto.
+*
 destruct si'; auto.
 unfold Ptrofs.of_intu in H.
-rewrite Ptrofs.to_int_of_int in H by auto.
-subst.
-unfold Ptrofs.of_ints.
-rewrite Int.signed_zero.
-unfold Ptrofs.to_int.
-rewrite Ptrofs.unsigned_repr.
-reflexivity.
-unfold Ptrofs.max_unsigned. rewrite (Ptrofs.modulus_eq32 Hp).
-compute; split; congruence.
+try ( (* Archi.ptr64=false case *)
+ rewrite Ptrofs.to_int_of_int in H by auto;
+ subst;
+ unfold Ptrofs.of_ints;
+ rewrite Int.signed_zero;
+ unfold Ptrofs.to_int;
+ rewrite Ptrofs.unsigned_repr; [reflexivity |];
+ unfold Ptrofs.max_unsigned; rewrite (Ptrofs.modulus_eq32 Hp);
+ compute; split; congruence).
+(* Archi.ptr64=true case *)
+unfold Ptrofs.of_int, Ptrofs.to_int64 in H;
+rewrite Ptrofs.unsigned_repr in H;
+ [apply Int64repr_Intunsigned_zero in H; subst; reflexivity
+ | pose proof (Int.unsigned_range i);
+   destruct H; split; auto;
+   assert (Int.modulus < Ptrofs.max_unsigned)
+     by (unfold Ptrofs.max_unsigned, Ptrofs.modulus, Ptrofs.wordsize, Wordsize_Ptrofs.wordsize; rewrite Hp; compute; auto);
+    omega].
+-
 destruct H.
 split; auto.
 hnf in H|-*. clear H0.
@@ -460,7 +491,7 @@ rewrite (Ptrofs.agree64_repr Hp) in H.
 rewrite Int64.repr_unsigned in H.
 apply Int64repr_Intunsigned_zero in H. subst.
 reflexivity.
-*
+-
 destruct H.
 split; auto.
 hnf in H|-*. clear H0.
@@ -471,6 +502,7 @@ rewrite (Ptrofs.agree32_repr Hp);
 rewrite Int.repr_unsigned in *;
 rewrite Int.repr_signed in *; rewrite Int.repr_unsigned in *; auto.
 Qed.
+
 
 Lemma test_order_fiddle_signed_xx:
  forall si si' v i phi, 
@@ -486,11 +518,22 @@ destruct H; split; auto.
 clear H.
 hnf in H0|-*.
 destruct si, si'; auto;
+try ( (* Archi.ptr64 = false *)
 unfold Ptrofs.to_int, Ptrofs.of_intu, Ptrofs.of_ints, Ptrofs.of_int in *;
 rewrite (Ptrofs.agree32_repr Hp) in H0;
 rewrite (Ptrofs.agree32_repr Hp);
 rewrite Int.repr_unsigned in *;
-rewrite Int.repr_signed in *; rewrite Int.repr_unsigned in *; auto.
+rewrite Int.repr_signed in *; rewrite Int.repr_unsigned in *; auto);
+try ((* Archi.ptr64 = true *)
+  unfold Ptrofs.to_int, Ptrofs.of_intu, Ptrofs.of_ints, Ptrofs.of_int in *;
+  unfold Ptrofs.to_int64 in *;
+  rewrite Ptrofs.unsigned_repr_eq in *;
+  change Ptrofs.modulus with Int64.modulus in *;
+  rewrite <- Int64.unsigned_repr_eq in *;
+  rewrite Int64.repr_unsigned in *;
+  first [apply Int64repr_Intsigned_zero in H0 
+          |apply Int64repr_Intunsigned_zero in H0];
+  subst i; reflexivity).
 Qed.
 
 Lemma test_order_fiddle_signed_yy:
@@ -507,11 +550,22 @@ destruct H; split; auto.
 clear H0.
 hnf in H|-*.
 destruct si, si'; auto;
+try ( (* Archi.ptr64 = false *)
 unfold Ptrofs.to_int, Ptrofs.of_intu, Ptrofs.of_ints, Ptrofs.of_int in *;
-rewrite (Ptrofs.agree32_repr Hp) in H;
+rewrite (Ptrofs.agree32_repr Hp) in H0;
 rewrite (Ptrofs.agree32_repr Hp);
 rewrite Int.repr_unsigned in *;
-rewrite Int.repr_signed in *; rewrite Int.repr_unsigned in *; auto.
+rewrite Int.repr_signed in *; rewrite Int.repr_unsigned in *; auto);
+try ((* Archi.ptr64 = true *)
+  unfold Ptrofs.to_int, Ptrofs.of_intu, Ptrofs.of_ints, Ptrofs.of_int in *;
+  unfold Ptrofs.to_int64 in *;
+  rewrite Ptrofs.unsigned_repr_eq in *;
+  change Ptrofs.modulus with Int64.modulus in *;
+  rewrite <- Int64.unsigned_repr_eq in *;
+  rewrite Int64.repr_unsigned in *;
+  first [apply Int64repr_Intsigned_zero in H 
+          |apply Int64repr_Intunsigned_zero in H];
+  subst i; reflexivity).
 Qed.
 
 Lemma denote_tc_nonzero_e':
@@ -618,8 +672,10 @@ Lemma denote_tc_iszero_long_e':
 Proof.
 intros.
 hnf in H.
-destruct (Int64.eq (Int64.repr (Int64.unsigned i)) Int64.zero);
-  auto; contradiction.
+pose proof (Int64.eq_spec i Int64.zero).
+destruct (Int64.eq i Int64.zero);
+  try contradiction.
+subst; reflexivity.
 Qed.
 
 Lemma eval_binop_relate':
